
\section*{Exercises for 3.13--3.14}

\begin{enumerate}
\item  Here is something obvious. If we have evidence that \p{P\lor Q} and we 
 have evidence that \p{\lnot P}, we have evidence that \p{Q}. Our proof system 
 confirms this. Add the missing datums in the following derivation:
%Derive from \p{\seq{\Gamma}{P \lor Q}} to \p{\seq{\Gamma, \Delta}{Q}}

\begin{argument*}
%generated by gentzen

\ai{\Gamma}{P \lor Q}{premise}

\ai{\Delta}{\lnot P}{premise}

\ai{P}{P}{A}

\ai{\mask{\Delta, \lnot Q}}{\lnot P}{2}

\ai{\mask{P, \lnot Q}}{P}{3}

\ai{\mask{\Delta, P}}{\lnot \lnot Q}{4,5,\negI}

\ai{\Delta, P}{Q}{6,\negE}

\ai{Q}{Q}{A}

\ai{\mask{\Gamma, \Delta}}{Q}{1,7,8,\disjE}

\end{argument*}



\item Derivations can often be adapted to prove something similar. For instance, 
 the above can be adapted easily to derive from \p{\seq{\Gamma}{\lnot P\lor Q}} 
 and \p{\seq{\Delta}{P}} to \p{\seq{\Gamma,\Delta}{Q}}. Fill in the missing 
 datums and annotations.

%Derive from \p{\seq{\Gamma}{\lnot P \lor Q}} to \p{\seq{\Gamma, \Delta}{Q}}

\begin{argument*}
%generated by gentzen

\ai{\Gamma}{\lnot P \lor Q}{premise}

\ai{\Delta}{P}{premise}

\ai{\mask{\lnot P}}{\lnot P}{A}

\ai{\mask{\Delta, \lnot Q}}{P}{2}

\ai{\mask{\lnot P, \lnot Q}}{\lnot P}{3}

\ai{\mask{\Delta, \lnot P}}{\lnot \lnot Q}{4,5,\negI}

\ai{\mask{\Delta, \lnot P}}{Q}{6,\negE}

\ai{Q}{Q}{A}

\ai{\mask{\Gamma, \Delta}}{Q}{1,7,8,\disjE}

\end{argument*}



 \newpage
\item The Greek capital letters on the datum side are place-holders. You can 
 plug anything you want into them. Take the derivation in Problem 2 above. You 
 can plug \p{P} into \p{\Delta} and add one more step at the end to show  that 
 you can infer from \p{\seq{\Gamma}{\lnot P \lor Q}} to \p{\seq{\Gamma}
 {P\limplies Q}} (which we should expect given the way the conditional is 
 defined).  Construct such a derivation.

 \answer{
%Derive from \p{\seq{\Gamma}{\lnot P \lor Q}} to \p{\seq{\Gamma}{P \limplies Q}}

\begin{argument*}
%generated by gentzen

\ai{\Gamma}{\lnot P \lor Q}{premise}

\ai{P}{P}{A}

\ai{\lnot P}{\lnot P}{A}

\ai{P, \lnot Q}{P}{2}

\ai{\lnot P, \lnot Q}{\lnot P}{3}

\ai{P, \lnot P}{\lnot \lnot Q}{4,5,\negI}

\ai{P, \lnot P}{Q}{6,\negE}

\ai{Q}{Q}{A}

\ai{\Gamma, P}{Q}{1,7,8,\disjE}

\ai{\Gamma}{P \limplies Q}{9,\condI}

\end{argument*}

 

 }

\item The following is a derivation from \p{\seq{\Gamma}{P\limplies Q}} to 
 \p{\seq{\Gamma}{\lnot P\lor Q}}. Again, we should expect that there is such a 
 derivation given the way the conditional was defined. Fill in the missing parts 
 of the derivation:

\begin{argument*}

\ai{\Gamma}{P \limplies Q}{premise}

\ai{\lnot (\lnot P \lor Q)}{\mask{\lnot (\lnot P \lor Q)}}{A}

\ai{\mask{\lnot P}}{\lnot P}{A}

\ai{\lnot P}{\lnot P \lor Q}{\mask{3,\disjI}}

\ai{\mask{\lnot (\lnot P \lor Q),\lnot P}}{\mask{\lnot (\lnot P \lor Q)}}{2}

\ai{\lnot (\lnot P \lor Q)}{\lnot \lnot P}{4,5,\negI}

\ai{\mask{\lnot (\lnot P \lor Q)}}{\mask{P}}{6,\negE}

\ai{\mask{\Gamma,\lnot (\lnot P \lor Q)}}{\mask{Q}}{1,7,\condE}

\ai{\Gamma,\lnot (\lnot P \lor Q)}{\lnot P \lor Q}{8,\disjI}

\ai{\Gamma}{\lnot \lnot (\lnot P \lor Q)}{\mask{2,9,\negI}}

\ai{\Gamma}{\lnot P \lor Q}{\mask{10,\negE}}

\end{argument*}

 \item Suppose there is evidence that \p{P \limplies Q}. In that case,  
  there is is evidence that \p{\lnot Q\limplies \lnot P}. Our proof system 
  confirms this. Construct a derivation from \p{\seq{\Gamma}{P\limplies Q}} 
  to \p{\seq{\Gamma}{\lnot Q\limplies \lnot P}}. Hint: you can adapt and modify 
  one the derivations given in Section 3.13.
\answer{
\begin{argument*}

\ai{\Gamma}{P \limplies Q}{premise}

\ai{\lnot Q}{\lnot Q}{A}

\ai{P}{P}{A}

\ai{\Gamma,P}{Q}{1,3,\condE}

\ai{\lnot Q,P}{\lnot Q}{2}

\ai{\Gamma,\lnot Q}{\lnot P}{4,5,\negI}

\ai{\Gamma}{\lnot Q \limplies \lnot P}{6,\condI}

\end{argument*}
}
\opts{\newpage}{}

\item Correct any errors in the annotations of the following derivation from 
 \lbh{-s /G:CPQ} and \lbh{-s /D:ARNQ} to \lbh{-s /G,/D:CPR} (the only errors are 
 in the annotations):



\begin{argumentN}[1]
%generated by gentzen

\ai{Γ}{P\mc{\limplies }Q}{premise}

\ai{Δ}{R\mc{\lor }\lnot Q}{\opts{A}{\textcircled{premise}}}

\ai{R}{R}{A}

\ai{R, P}{R}{3}

\ai{R}{P\mc{\limplies }R}{\opts{}{\textcircled{4,}}\condI}

\ai{\mc{\lnot }Q}{\mc{\lnot }Q}{\opts{2,4,\disjE}{\textcircled{A}}}

\ai{P}{P}{A}

\ai{Γ, P}{Q}{1,7,\opts{\conjE}{\textcircled{\condE}}}

\ai{\mc{\lnot }Q, P}{\mc{\lnot }Q}{6}

\ai{Γ, \mc{\lnot }Q}{\mc{\lnot }P}{\opts{6,8}{\textcircled{8,9}},\negI}

\ai{Γ, \mc{\lnot }Q}{\lnot P\mc{\lor }R}{\opts{7,10}{\textcircled{10}},\disjI}

\ai{\mc{\lnot }P}{\mc{\lnot }P}{A}

\ai{\mc{\lnot }P, \mc{\lnot }R}{\mc{\lnot }P}{\opts{11,3,\condE}
{\textcircled{12}}}

\ai{P, \mc{\lnot }R}{P}{\opts{10}{\textcircled{7}}}

 \ai{\mc{\lnot }P, P}{\mc{\lnot }\lnot R}{13,14,\opts{\negE}
 {\textcircled{\negI}}}

 \ai{\mc{\lnot }P, P}{R}{15,\opts{\negI}{\textcircled{\negE}}}

 \ai{\mc{\lnot }P}{P\mc{\limplies }R}{16,\opts{\conjI}{\textcircled{\condI}}}

\ai{Γ, \mc{\lnot }Q}{P\mc{\limplies }R}{11,17,5,\disjE}

\ai{Γ, Δ}{P\mc{\limplies }R}{\opts{2,5,17,18}{\textcircled{2,5,18}},\disjE}

\end{argumentN}

 \item If you have evidence that \p{(W\lor Y)\limplies Z}, you have evidence 
  that \p{W\limplies Z}. Construct a derivation from \p{\seq{\Gamma}{(W\lor Y)
	\limplies Z}} to \p{\seq{\Gamma}{W\limplies Z}}.

\answer{
\begin{argument*}

\ai{\Gamma}{(W \lor Y) \limplies Z}{premise}

\ai{W}{W}{A}

\ai{W}{W \lor Y}{2,\disjI}

\ai{\Gamma,W}{Z}{1,3,\condE}

\ai{\Gamma}{W \limplies Z}{4,\condI}

\end{argument*}

}
\end{enumerate}


