\section*{Exercises for 5.12--5.14}

\begin{enumerate}
 \setlength{\itemsep}{2em}

 \item Add missing items:


\begin{argumentN}[1]
%generated by gentzen

\ai{\lforall x Fx\mc{\land }\lforall x Gx}{\lforall x Fx\mc{\land }\lforall x Gx}
{\mask{A}}

\ai{\lforall x Fx\mc{\land }\lforall x Gx}{\mc{\lforall x }Fx}{\mask{1,\conjE}}

\ai{\lforall x Fx\mc{\land }\lforall x Gx}{Fa}{\mask{2,\uniE}}

\ai{\lforall x Fx\mc{\land }\lforall x Gx}{\mc{\lforall x }Gx}{\mask{1,\conjE}}

\ai{\lforall x Fx\mc{\land }\lforall x Gx}{Gb}{\mask{4,\uniE}}

\ai{\lforall x Fx\mc{\land }\lforall x Gx}{Fa\mc{\land }Gb}{\mask{3,5,\conjI}}

\ai{\lforall x Fx\mc{\land }\lforall x Gx}{\mc{\lforall y }(Fa\land Gy)}{\mask{6,
\uniI}}

\ai{\lforall x Fx\mc{\land }\lforall x Gx}{\mc{\lforall x }\lforall y (Fx\land 
Gy)}{\mask{7,\uniI}}

\end{argumentN}

\item Prove \lbh{-p -s UxKFxUyGy:UxUyKFxGy}. Hint: compare with proof 
 above.
\opts{
   \dotline
   \dotline
   \dotline
   \dotline
   \dotline
   \dotline
   \dotline
   \dotline
   \dotline
   \dotline
   \dotline
  }
  {

\begin{argumentN}[1]
%generated by gentzen

\ai{\mc{\lforall x }(Fx\land \lforall y Gy)}{\mc{\lforall x }(Fx\land \lforall y Gy)}{A}

\ai{\mc{\lforall x }(Fx\land \lforall y Gy)}{Fa\mc{\land }\lforall y Gy}{1,\uniE}

\ai{\mc{\lforall x }(Fx\land \lforall y Gy)}{Fa}{2,\conjE}

\ai{\mc{\lforall x }(Fx\land \lforall y Gy)}{\mc{\lforall y }Gy}{2,\conjE}

\ai{\mc{\lforall x }(Fx\land \lforall y Gy)}{Gb}{4,\uniE}

\ai{\mc{\lforall x }(Fx\land \lforall y Gy)}{Fa\mc{\land }Gb}{3,5,\conjI}

\ai{\mc{\lforall x }(Fx\land \lforall y Gy)}{\mc{\lforall y }(Fa\land Gy)}{6,\uniI}

\ai{\mc{\lforall x }(Fx\land \lforall y Gy)}{\mc{\lforall x }\lforall y (Fx\land Gy)}{7,\uniI}

\end{argumentN}

  }
\newpage

  \item Add missing items:



\begin{argumentN}[1]
%generated by gentzen

\ai{\lforall x Fx\mc{\lor }\lforall x Gx}{\lforall x Fx\mc{\lor }\lforall x Gx}{A}

\ai{\mc{\lforall x }Fx}{\mc{\lforall x }Fx}{A}

\ai{\mc{\lforall x }Fx}{\mask{Fa}}{2,\uniE}

\ai{\mc{\lforall x }Fx}{\mask{Fa\mc{\lor }Gb}}{3,\disjI}

\ai{\mask{\mc{\lforall x }Gx}}{\mask{\mc{\lforall x }Gx}}{A}

\ai{\mask{\mc{\lforall x }Gx}}{Gb}{\mask{5,\uniE}}

\ai{\mask{\mc{\lforall x }Gx}}{\mask{Fa\mc{\lor }Gb}}{\mask{6,\disjI}}

\ai{\lforall x Fx\mc{\lor }\lforall x Gx}{Fa\mc{\lor }Gb}{1,4,7,\disjE}

\ai{\lforall x Fx\mc{\lor }\lforall x Gx}{\mc{\lforall y }(Fa\lor Gy)}{\mask{8,
\uniI}}

\ai{\lforall x Fx\mc{\lor }\lforall x Gx}{\mc{\lforall x }\lforall y (Fx\lor Gy)}
{\mask{9,\uniI}}

\end{argumentN}


  \item Prove \lbh{-p -s UxAFxUyGy:UxUyAFxGy}. 

   \opts{
   \dotline
   \dotline
   \dotline
   \dotline
   \dotline
   \dotline
   \dotline
   \dotline
   \dotline
   \dotline
   \dotline
  }
  {


\begin{argumentN}[1]
%generated by gentzen

\ai{\mc{\lforall x }(Fx\lor \lforall y Gy)}{\mc{\lforall x }(Fx\lor \lforall y Gy)}{A}

\ai{\mc{\lforall x }(Fx\lor \lforall y Gy)}{Fa\mc{\lor }\lforall y Gy}{1,\uniE}

\ai{Fa}{Fa}{A}

\ai{Fa}{Fa\mc{\lor }Gb}{3,\disjI}

\ai{\mc{\lforall y }Gy}{\mc{\lforall y }Gy}{A}

\ai{\mc{\lforall y }Gy}{Gb}{5,\uniE}

\ai{\mc{\lforall y }Gy}{Fa\mc{\lor }Gb}{6,\disjI}

\ai{\mc{\lforall x }(Fx\lor \lforall y Gy)}{Fa\mc{\lor }Gb}{2,4,7,\disjE}

\ai{\mc{\lforall x }(Fx\lor \lforall y Gy)}{\mc{\lforall y }(Fa\lor Gy)}{8,\uniI}

\ai{\mc{\lforall x }(Fx\lor \lforall y Gy)}{\mc{\lforall x }\lforall y (Fx\lor Gy)}{9,\uniI}

\end{argumentN}

}
   \newpage

  \item Prove  \lbh{-p -s KUxFxXxGx:UxXyKFxGy}. Here are the first few 
   lines:

	\begin{argumentN}[1]
\ai{\lforall x Fx\mc{\land }\lthereis x Gx}{\lforall x Fx\mc{\land }\lthereis x 
Gx}{A}

\ai{\lforall x Fx\mc{\land }\lthereis x Gx}{\mc{\lforall x }Fx}{1,\conjE}

\ai{\lforall x Fx\mc{\land }\lthereis x Gx}{Fa}{2,\uniE}

\ai{\lforall x Fx\mc{\land }\lthereis x Gx}{\mc{\lthereis x }Gx}{1,\conjE}

\ai{Gb}{Gb}{A}

  \end{argumentN} 

  \opts{

   \dotline
   \dotline
   \dotline
   \dotline
   \dotline
   \dotline
  }
  {
\vskip 1em
\begin{argumentN}[6]

 \ai[0.3]{\lforall x Fx\mc{\land }\lthereis x Gx, Gb}{Fa\mc{\land }Gb}{3,5,
 \conjI}

\ai[0.3]{\lforall x Fx\mc{\land }\lthereis x Gx, Gb}{\mc{\lthereis y }(Fa\land Gy)}{6,\exI}

\ai[0.3]{\lforall x Fx\mc{\land }\lthereis x Gx, Gb}{\mc{\lforall x }\lthereis y (Fx\land Gy)}{7,\uniI}

\ai[0.3]{\lforall x Fx\mc{\land }\lthereis x Gx}{\mc{\lforall x }\lthereis y (Fx\land Gy)}{4,8,\exE}

\end{argumentN}

}


  \item Prove \lbh{-p -s KUxFxNUxGx:UxXyKFxNGy}. Hint: Use Quantifer 
   Exchange to get rid of the negation in front of the universal quantifier; you 
   will get something that looks very much like one of the problems above.
\opts{

   \dotline
   \dotline
   \dotline
   \dotline
   \dotline
   \dotline
   \dotline
   \dotline
   \dotline
   \dotline
   \dotline
   \dotline
   \dotline

  }
  {
 

\begin{argumentN}[1]
%generated by gentzen

\ai[0.35]{\lforall x Fx\mc{\land }\lnot \lforall x Gx}{\lforall x Fx\mc{\land }\lnot \lforall x Gx}{A}

\ai[0.35]{\lforall x Fx\mc{\land }\lnot \lforall x Gx}{\mc{\lnot }\lforall x Gx}{1,\conjE}

\ai[0.35]{}{\lnot \lforall x Gx\mc{\limplies }\lthereis x \lnot Gx}{QE}

\ai[0.35]{\lforall x Fx\mc{\land }\lnot \lforall x Gx}{\mc{\lthereis x }\lnot Gx}{2,3,\condE}

\ai[0.35]{\mc{\lnot }Gb}{\mc{\lnot }Gb}{A}

\ai[0.35]{\lforall x Fx\mc{\land }\lnot \lforall x Gx}{\mc{\lforall x }Fx}{1,\conjE}

\ai[0.35]{\lforall x Fx\mc{\land }\lnot \lforall x Gx}{Fa}{6,\uniE}

\ai[0.35]{\lforall x Fx\mc{\land }\lnot \lforall x Gx, \mc{\lnot }Gb}{Fa\mc{\land }\lnot Gb}{5,7,\conjI}

\ai[0.35]{\lforall x Fx\mc{\land }\lnot \lforall x Gx, \mc{\lnot }Gb}{\mc{\lthereis y }(Fa\land \lnot Gy)}{8,\exI}

\ai[0.35]{\lforall x Fx\mc{\land }\lnot \lforall x Gx, \mc{\lnot }Gb}{\mc{\lforall x }\lthereis y (Fx\land \lnot Gy)}{9,\uniI}

\ai[0.35]{\lforall x Fx\mc{\land }\lnot \lforall x Gx}{\mc{\lforall x }\lthereis y (Fx\land \lnot Gy)}{4,10,\exE}

\end{argumentN}


  }
  \cover{\newpage}
 \item Here is something obvious: if there are at least two Fs, there is at 
  least one F.  Let's make sure that our way of counting delivers this result.  
  Prove \lbh{-p -s XxKFxXyKGyN=xy:XxFx}. Hint: for how to do the first few 
  lines, consider the next problem.

  \opts{
   \dotline
   \dotline
   \dotline
   \dotline
   \dotline
   \dotline
   \dotline
   \dotline
   \dotline
  }
  {
\small
\begin{argumentN}[1]
%generated by gentzen

\ai[0.37]{\mc{\lthereis x }[Fx\land \lthereis y (Gy\land \nident{x}{y})]}
{\mc{\lthereis x }[Fx\land \lthereis y (Gy\land \nident{x}{y})]}{A}

\ai[0.35]{Fa\mc{\land }\lthereis y (Gy\land \nident{a}{y})}{Fa\mc{\land }\lthereis y (Gy\land \nident{a}{y})}{A}

\ai[0.35]{Fa\mc{\land }\lthereis y (Gy\land \nident{a}{y})}{Fa}{2,\conjE}

\ai[0.35]{Fa\mc{\land }\lthereis y (Gy\land \nident{a}{y})}{\mc{\lthereis x }Fx}{3,\exI}

\ai[0.4]{\mc{\lthereis x }[Fx\land \lthereis y (Gy\land \nident{x}{y})]}
{\mc{\lthereis x }Fx}{1,4,\exE}

\end{argumentN}

}
\item Prove \lbh{-p -s XxKFxXyGy:XxXyKFxGy}. Here are the first few lines.
\begin{argumentN}[1]
%generated by gentzen

 \ai[0.25]{\mc{\lthereis x }(Fx\land \lthereis y Gy)}{\mc{\lthereis x }(Fx\land 
 \lthereis y Gy)}{A}

\ai[0.25]{Fa\mc{\land }\lthereis y Gy}{Fa\mc{\land }\lthereis y Gy}{A}

\ai[0.25]{Fa\mc{\land }\lthereis y Gy}{Fa}{2,\conjE}

\ai[0.25]{Fa\mc{\land }\lthereis y Gy}{\mc{\lthereis y }Gy}{2,\conjE}

\end{argumentN}
\opts{
\dotline
\dotline
\dotline
\dotline
\dotline
\dotline
\dotline
\dotline
\dotline
}
{
 \vskip 1em
 \begin{argumentN}[5]
\ai[0.3]{Gb}{Gb}{A}

\ai[0.3]{Fa\mc{\land }\lthereis y Gy, Gb}{Fa\mc{\land }Gb}{3,5,\conjI}

\ai[0.3]{Fa\mc{\land }\lthereis y Gy, Gb}{\mc{\lthereis y }(Fa\land Gy)}{6,\exI}

\ai[0.3]{Fa\mc{\land }\lthereis y Gy, Gb}{\mc{\lthereis x }\lthereis y (Fx\land Gy)}{7,\exI}

\ai[0.3]{Fa\mc{\land }\lthereis y Gy}{\mc{\lthereis x }\lthereis y (Fx\land Gy)}{4,8,\exE}

\ai[0.3]{\mc{\lthereis x }(Fx\land \lthereis y Gy)}{\mc{\lthereis x }\lthereis y (Fx\land Gy)}{1,9,\exE}

\end{argumentN}

}{
}
\newpage

  \item In Section 5.14 I claim without explanation that formulas 4 and 5 say 
   the same thing. If I am right, we expect a derivation from formula 4 to 
   formula 5.  Here is a such a derivation. Add missing items (note: 
   \lbh{-p -f NN=ab} is the same as \p{\lnot\lnot(\ident{a}{b})}):

   To aid visibility, let 

   \begin{itemize}

  \item[\p{\Gamma}:]  \p{\lthereis x[Fx\land\lnot\lthereis y(Fy\land\nident{x}
  {y})]} 

 \item[\p{\Delta}:]   \p{Fa\land  \lnot \lthereis y (Fy\land \nident{a}
   {y})]}


\end{itemize}
Notice \p{\Delta} has a constant so we need to be mindful of that.
\begin{argumentN}[1]
%generated by gentzen

\ai[0.15]{\Gamma}
{\mc{\lthereis x }[Fx\land \lnot \lthereis y (Fy\land \nident{x}{y})]}{A}

\ai[0.15]{\Delta}{Fa\mc{\land }\lnot \lthereis y (Fy\land \nident{a}{y})}{A}

\ai[0.15]{\Delta}{\mask{\mc{\lnot }\lthereis y (Fy\land \nident{a}{y})}}{2,
 \conjE}

\ai[0.15]{}{\mask{\lnot \lthereis y (Fy\land \nident{a}{y})\mc{\limplies }
\lforall y \lnot (Fy\land \nident{a}{y})}}{QE}

\ai[0.15]{\Delta}{\mc{\lforall y }\lnot (Fy\land \nident{a}{y})}{3,4,\condE}

\ai[0.15]{\Delta}{\mask{\mc{\lnot }(Fb\land \nident{a}{b})}}{5,\uniE}

\ai[0.15]{}{\lnot (Fb\land \nident{a}{b})\mc{\limplies }[\lnot Fb\lor \lnot (\nident{a}{b})]}{DM}

\ai[0.15]{\Delta}{\mask{\lnot Fb\mc{\lor }\lnot (\nident{a}{b})}}{6,7,\condE}

\ai[0.15]{}{[\lnot Fb\lor \lnot (\nident{a}{b})]\mc{\limplies }[\lnot \lnot Fb\limplies \lnot (\nident{a}{b})]}{EL}

\ai[0.15]{\mask{\Delta}}{\mask{\lnot \lnot Fb\mc{\limplies }\lnot (\nident{a}
{b})}}
{8,
 9,
\condE}

\ai[0.15]{Fb}{Fb}{A}

\ai[0.15]{}{Fb\mc{\limplies }\lnot \lnot Fb}{DN}

\ai[0.15]{Fb}{\mc{\lnot }\lnot Fb}{\mask{11,12,\condE}}

\ai[0.15]{\Delta, Fb}{\mc{\lnot }(\nident{a}{b})}{10,13,\condE}

\ai[0.15]{\Delta, Fb}{\ident{a}{b}}{\mask{14,\negE}}

\ai[0.15]{\mask{\Delta}}{\mask{Fb\mc{\limplies }\ident{a}{b}}}{15,\condI}

\ai[0.15]{\Delta}{\mask{\mc{\lforall y }(Fy\limplies \ident{a}{y})}}{16,\uniI}

\ai[0.15]{\Delta}{\mask{Fa}}{\mask{2,\conjE}}

\ai[0.15]{\Delta}{Fa\mc{\land }\lforall y (Fy\limplies \ident{a}{y})}{17,18,\conjI}

\ai[0.15]{\mask{\Delta}}{\mc{\lthereis x }[Fx\land \lforall y (Fy\limplies 
 \ident{x}
{y})]}{19,\exI}

\ai[0.15]{\Gamma}{\mc{\lthereis x }[Fx\land \lforall y (Fy\limplies \ident{x}
{y})]}{\mask{1,20,\exE}}

\end{argumentN}


\item Here is another way of saying that there is exactly one thing:

 \lbh{-p -f  XxUyKFxCFy=xy}

 Prove \lbh{-p -s XxKFxUyCFy=xy:XxUyKFxCFy=xy}. Here are the first two 
 lines:

 \begin{argumentN}[1]
%generated by gentzen

 \ai[0.35]{\mc{\lthereis x }[Fx\land \lforall y (Fy\limplies \ident{x}{y})]}
{\mc{\lthereis x }[Fx\land \lforall y (Fy\limplies \ident{x}{y})]}{A}

\ai[0.35]{Fa\mc{\land }\lforall y (Fy\limplies \ident{a}{y})}{Fa\mc{\land }
\lforall y (Fy\limplies \ident{a}{y})}{A}

\end{argumentN}
\opts{
\dotline
\dotline
\dotline
\dotline
\dotline
\dotline
\dotline
\dotline
\dotline
}{
\small
 \vskip 1em
\begin{argumentN}[3]

\ai[0.35]{Fa\mc{\land }\lforall y (Fy\limplies \ident{a}{y})}{Fa}{2,\conjE}

\ai[0.35]{Fa\mc{\land }\lforall y (Fy\limplies \ident{a}{y})}{\mc{\lforall y }(Fy\limplies \ident{a}{y})}{2,\conjE}

\ai[0.35]{Fa\mc{\land }\lforall y (Fy\limplies \ident{a}{y})}{Fb\mc{\limplies }\ident{a}{b}}{4,\uniE}

\ai[0.35]{Fa\mc{\land }\lforall y (Fy\limplies \ident{a}{y})}{Fa\mc{\land }(Fb\limplies \ident{a}{b})}{3,5,\conjI}

\ai[0.35]{Fa\mc{\land }\lforall y (Fy\limplies \ident{a}{y})}{\mc{\lforall y }[Fa\land (Fy\limplies \ident{a}{y})]}{6,\uniI}

\ai[0.35]{Fa\mc{\land }\lforall y (Fy\limplies \ident{a}{y})}{\mc{\lthereis x }\lforall y [Fx\land (Fy\limplies \ident{x}{y})]}{7,\exI}

\ai[0.35]{\mc{\lthereis x }[Fx\land \lforall y (Fy\limplies \ident{x}{y})]}{\mc{\lthereis x }\lforall y [Fx\land (Fy\limplies \ident{x}{y})]}{1,8,\exE}

\end{argumentN}

}

\item Prove \lbh{-p -s XxUyKFxGy:XxKFxUyGy}. (This is a simplified version 
 of the reverse of the above).

 \opts{

  \dotline
\dotline
\dotline
\dotline
\dotline
\dotline
\dotline
\dotline
\dotline
\dotline
\dotline
\dotline
}
{
\begin{argumentN}[1]
%generated by gentzen

\ai[0.25]{\mc{\lthereis x }\lforall y (Fx\land Gy)}{\mc{\lthereis x }\lforall y (Fx\land Gy)}{A}

\ai[0.25]{\mc{\lforall y }(Fa\land Gy)}{\mc{\lforall y }(Fa\land Gy)}{A}

\ai[0.25]{\mc{\lforall y }(Fa\land Gy)}{Fa\mc{\land }Gb}{2,\uniE}

\ai[0.25]{\mc{\lforall y }(Fa\land Gy)}{Gb}{3,\conjE}

\ai[0.25]{\mc{\lforall y }(Fa\land Gy)}{\mc{\lforall y }Gy}{4,\uniI}

\ai[0.25]{\mc{\lforall y }(Fa\land Gy)}{Fa}{3,\conjE}

\ai[0.25]{\mc{\lforall y }(Fa\land Gy)}{Fa\mc{\land }\lforall y Gy}{5,6,\conjI}

\ai[0.25]{\mc{\lforall y }(Fa\land Gy)}{\mc{\lthereis x }(Fx\land \lforall y Gy)}{7,\exI}

\ai[0.25]{\mc{\lthereis x }\lforall y (Fx\land Gy)}{\mc{\lthereis x }(Fx\land \lforall y Gy)}{1,8,\exE}

\end{argumentN}

}

\end{enumerate}

